Horrible checkpoint of a merge.

src/ml/libvellvm/interpreter.mli
@@ -1,0 +1,13 @@
+;; open TopLevel.IO
+
+val pp_addr : Format.formatter -> Memory.A.addr -> unit
+
+val pp_dvalue : Format.formatter -> DV.dvalue -> unit
+
+val interpret: ((LLVMAst.block list) LLVMAst.toplevel_entity list) -> (DV.dvalue, string) result
+
+(* SAZ: do we need to expose the step function in this way?  Its type is very complicated *)
+(* val step : ((Obj.t Std.failureE, Obj.t debugE, 'b) Sum.sum1, DV.dvalue) coq_LLVM -> (TopLevel.IO.DV.dvalue, string) result *)
+val step : ((Obj.t failureE, Obj.t debugE, 'b) Sum.sum1, 'a * DV.dvalue) coq_LLVM -> (TopLevel.IO.DV.dvalue, string) result
+
+val debug_flag: bool ref
