src/ml/test.ml
@@ -19,7 +19,7 @@
 
 let parse_pp_test path =
   let _ = Platform.verb @@ Printf.sprintf "* processing file: %s\n" path in
-  let filename, ext = Platform.path_to_basename_ext path in
+  let filename, _ = Platform.path_to_basename_ext path in
   let vll_file = Platform.gen_name !Platform.output_path filename ".v.ll" in
   let dot_s = Platform.gen_name !Platform.output_path filename ".s" in
   let _ = Printf.fprintf stderr "Running llc on: %s\n%!" path in
@@ -59,7 +59,12 @@ let pp_test_of_dir dir =
         List.map (fun f -> (f, fun () -> parse_pp_test f)) (files_of_dir dir))
 
 let run_dvalue_test (test:IO.DV.dvalue -> bool) path =
-  if not (test (run_ll_file path)) then failwith (path ^ " test failed"); ()
+  let (res, msg) =
+    match run_ll_file path with
+    | Error msg -> (false, msg)
+    | Ok dv -> (test dv, "")
+  in
+  if not res then failwith (path ^ " test failed: " ^ msg); ()
 
 let poison_tests =
   ["../tests/llvm-arith/i1/add_nsw.ll";
@@ -135,7 +140,22 @@ let i64_tests : (string * int) list =
     ("../tests/ll/gep8.ll", 2);
     ("../tests/ll/gep9.ll", 5);
   ]
-    
+
+let float_tests : (string * float ) list =
+  [
+    ("../tests/llvm-arith/float/i8_uitofp_float.ll", 10.0)
+  ]
+
+let double_tests : (string * float ) list =
+  [
+    ("../tests/llvm-arith/double/i8_uitofp_double.ll", 255.0)
+  ]
+
+let intrinsics_tests : (string * float) list =
+  [
+    ("../tests/intrinsics/llvm_fabs_f64.ll", 1.0)
+  ]
+
 let parse_files =
   [  ]
 
@@ -144,7 +164,10 @@ let test_dirs =
    "../tests/llvm-arith/i1/";
    "../tests/llvm-arith/i8/";
    "../tests/llvm-arith/i32/";
-   "../tests/llvm-arith/i64/"]
+   "../tests/llvm-arith/i64/";
+   "../tests/llvm-arith/float/";
+   "../tests/llvm-arith/double/";
+  ]
 
 let poison_test = function
   | IO.DV.DVALUE_Poison -> true
@@ -174,6 +197,19 @@ let i64_test (i1:int64) = function
      Int64.eq i1 i2
   | _ -> false
 
+(* NOTE: OCaml's floats are actually 64-bit doubles, but contain 32-bit floats as a subset *)
+let float_test (i1:float) = function
+  | IO.DV.DVALUE_Float i2 ->
+    compare i1 (Camlcoq.camlfloat_of_coqfloat32 i2) = 0
+  | _ -> false
+
+let double_test (i1:float) = function
+  | IO.DV.DVALUE_Double i2 ->
+    compare i1 (Camlcoq.camlfloat_of_coqfloat i2) = 0
+  | _ -> false
+
+
+
 let i1_of_int i = Int1.repr (Camlcoq.Z.of_sint i)
 
 let i8_of_int i = Int8.repr (Camlcoq.Z.of_sint i)
@@ -182,20 +218,48 @@ let i32_of_int i = Int32.repr (Camlcoq.Z.of_sint i)
 
 let i64_of_int i = Int64.repr (Camlcoq.Z.of_sint i)
                                             
-let suite = [Test ("Parsing", List.map (fun f -> (f, fun () -> parse_pp_test f)) parse_files);
-             Test ("Poison", List.map (fun f ->
-                                 (f, fun () -> run_dvalue_test poison_test f)) poison_tests);
-             Test ("I1-arith", List.map (fun (f, i) ->
-                                   (f, fun () -> run_dvalue_test (i1_test (i1_of_int i)) f))
-                                        i1_tests);
-             Test ("I8-arith", List.map (fun (f, i) ->
-                                   (f, fun () -> run_dvalue_test (i8_test (i8_of_int i)) f))
-                                        i1_tests);
-             Test ("I32-arith", List.map (fun (f, i) ->
-                                    (f, fun () -> run_dvalue_test (i32_test (i32_of_int i)) f))
-                                         i32_tests);
-             Test ("I64-arith", List.map (fun (f, i) ->
-                                    (f, fun () -> run_dvalue_test (i64_test (i64_of_int i)) f))
-                                         i64_tests)] @
+let suite = [Test ("Poison",
+                   List.map (fun f ->
+                       (f, fun () -> run_dvalue_test poison_test f))
+                     poison_tests);
+
+             Test ("I1-arith",
+                   List.map (fun (f, i) ->
+                       (f, fun () -> run_dvalue_test (i1_test (i1_of_int i)) f))
+                     i1_tests);
+
+             Test ("I8-arith",
+                   List.map (fun (f, i) ->
+                       (f, fun () -> run_dvalue_test (i8_test (i8_of_int i)) f))
+                     i1_tests);
+
+             Test ("I32-arith",
+                   List.map (fun (f, i) ->
+                       (f, fun () -> run_dvalue_test (i32_test (i32_of_int i)) f))
+                     i32_tests);
+
+             Test ("I64-arith",
+                   List.map (fun (f, i) ->
+                       (f, fun () -> run_dvalue_test (i64_test (i64_of_int i)) f))
+                     i64_tests);
+
+             Test ("Float-arith",
+                   List.map (fun (f, i) ->
+                       (f, (fun () -> run_dvalue_test (float_test i) f)))
+                       float_tests);
+
+             Test ("Double-arith",
+                   List.map (fun (f, i) ->
+                       (f, (fun () -> run_dvalue_test (double_test i) f)))
+                       double_tests);
+
+             Test ("Intrinsics",
+                   List.map (fun (f, i) ->
+                       (f, (fun () -> run_dvalue_test (double_test i) f)))
+                       intrinsics_tests);
+            ]
+
+
+            @
               (List.map pp_test_of_dir test_dirs)
 
