src/coq/CFGProp.v
@@ -10,8 +10,8 @@
 
 Require Import ZArith List String Omega.
 Require Import Vellvm.LLVMAst Vellvm.CFG Vellvm.Dom.
-Require Import Vellvm.Classes.
 Require Vellvm.AstLib.
+
 Import ListNotations.
 Open Scope list_scope.
 
@@ -155,7 +155,8 @@ Fixpoint exp_uses (v:exp) : list ident :=
   match v with
   | EXP_Ident id => [id]
   | EXP_Integer _
-  | EXP_Float _ 
+  | EXP_Float _
+  | EXP_Double _               
   | EXP_Hex _        
   | EXP_Bool _
   | EXP_Null
@@ -197,6 +198,7 @@ Definition instr_uses (i:instr) : (list ident) :=
   | INSTR_Alloca t (Some tv) align => texp_uses tv
   | INSTR_Load  volatile t ptr align => texp_uses ptr
   | INSTR_Store volatile val ptr align => (texp_uses val) ++ (texp_uses ptr)
+  | INSTR_Comment _
   | INSTR_Fence 
   | INSTR_AtomicCmpXchg
   | INSTR_AtomicRMW
@@ -288,7 +290,7 @@ Definition def_at_pt (g:cfg) (p:pt) (lid:local_id) : Prop :=
 
 (** The definition of id dominates its use at point pt *)
 Inductive well_scoped_use_at_pt (g:cfg) (p:pt) : ident -> Prop :=
-| ws_global : forall id, In id (glbl g) -> pt_exists g p -> well_scoped_use_at_pt g p id
+| ws_global : forall id, In id (glbl g) -> pt_exists g p -> well_scoped_use_at_pt gy p id
 | ws_local : forall lid p', def_at_pt g p' lid -> SDom g p' p -> well_scoped_use_at_pt g p (ID_Local lid).
 
 (** All uses of a [uid] must be strictly dominated by their definitions. *)
