README.md
@@ -51,27 +51,33 @@ University of Pennsylvania as part of the DeepSpec project.
 
 ### Assumes: 
   - coqc   : version 8.8.0   (and coqdep, etc.)
-  - Coq packages: ext-lib    (installed via, e.g. opam install coq-ext-lib)
-  - ocamlc : version 4.04    (probably works with 4.02 or later)
-  - OPAM packages: ocamlbuild, menhir, [optional: llvm  (for llvm v. 3.8)]
+  - Coq packages: 
+    - ext-lib    (installed via, e.g. opam install coq-ext-lib)
+    - paco       (installed via, e.g. opam install coq-paco)
+    - flocq      (installed via, e.g. opam install coq-flocq, see note below) 
+    - itree      (installed via, e.g. opam install coq-itree)
+- ocamlc : version 4.04    (probably works with 4.03 or later)
+  - OPAM packages: dune, menhir, [optional: llvm  (for llvm v. 3.8)]
 
 Compilation:
 
 1. clone the vellvm git repo with `--recurse-submodule` option (`git clone --recurse-submodules`)
-2. update CompCert submodule to coq 8.7.1 compatible version:
-   1. `cd lib/CompCert && git pull origin master`
-3. compile 3rd party libraries:
-   1. CompCert: `cd lib/Compcert && ./configure x86_64-macosx && make`
-   2. Compile Paco: `make -C lib/paco/src`
-   3. Compile InteractionTrees
-      - create the file `lib/InteractionTrees/_CoqPath` and edit it to contain
-      `-Q ../paco/src Paco`
-	  - run `make` from the InteractionTrees directory  (do _not_ use `setup.sh`
-        since that will clone another copy of paco and we already assume ext-lib exists)
-4. run `make` in the /src directory
+2. run `make` in the /src directory
 
 # Running
 
 Do `src/vellvm -help` from the command line.
 
 Try `src/vellvm -interpret tests/ll/factorial.ll`.
+
+
+# Notes
+
+### coq-flocq
+
+On some OSX configurations the opam installation for coq-flocq fails with a
+permissions error `# Failed to create server: Operation not permitted` caused by
+opam's sandboxing scripts.  The solution is to temporarily disable opam's
+sandboxing by editing ~/.opam/config to remove the lines having to do with
+`wrap-*-commands:`.
+
